Lp2lc/Next/STLC/__Infer_Umbral.lean
@@ -8,15 +8,15 @@ namespace Umbral
 
 section variable [env : ProvingBase]
 
-structure SafetyOf (trm : AST.Trm env.BuildF) where
-  typ : AST.Typ env.BuildF
+structure SafetyOf (trm : AST.Trm env.BuildParameters) where
+  typ : AST.Typ env.BuildParameters
   -- safety : Safety trm typ -- TODO: this lemma has been temporarily disabled. Enable it later.
 
-abbrev Compilation (trm : AST.Trm env.BuildF) :=
+abbrev Compilation (trm : AST.Trm env.BuildParameters) :=
   Rec.OutcomeOpt (SafetyOf trm) -- one observation of the semi-decidability of executing term
 
 /-- Requires the proving computation to shadow term inference at the selected fuel. -/
-structure Objective (trm : AST.Trm env.BuildF) (fuel : Nat) : Type 2 where
+structure Objective (trm : AST.Trm env.BuildParameters) (fuel : Nat) : Type 2 where
   compilation : Compilation trm
   sameInfer : compilation.map (Option.map SafetyOf.typ) = trm.infer fuel
 
